Coq. Proved lemmas about lbl_step.

Coq/src/LblStep.v
@@ -2,6 +2,7 @@ Require Import Omega.
 From hahn Require Import Hahn.
 From imm Require Import Events Execution
      Prog ProgToExecution ProgToExecutionProperties.
+Require Import AuxRel.
 
 Lemma unique_eps_step thread state state' state''
       (EPS_STEP1 : istep thread [] state state')
@@ -75,6 +76,9 @@ Definition ineps_step thread lbls (state state' : state) :=
   ⟪ NNIL : lbls <> [] ⟫ /\
   ⟪ STEP : istep thread lbls state state' ⟫.
 
+Definition neps_step thread (state state' : state) :=
+  exists lbls, ineps_step thread lbls state state'.
+
 Definition ilbl_step thread lbls :=
   ineps_step thread lbls ⨾ (istep thread [])＊ ⨾ ⦗ stable_state thread ⦘.
 
@@ -102,20 +106,73 @@ Qed.
 Lemma ilbl_steps_in_steps thread : (lbl_step thread)＊ ⊆ (step thread)＊.
 Proof. rewrite lbl_step_in_steps. apply rt_of_ct. Qed.
 
-Lemma ineps_step_dom_stable thread lbls :
-  ineps_step thread lbls ⊆ ⦗ stable_state thread ⦘ ⨾ ineps_step thread lbls.
+Lemma ineps_eps_step_dom_empty thread lbls :
+  dom_rel (ineps_step thread lbls) ∩₁ dom_rel (istep thread []) ≡₁ ∅.
 Proof.
-  intros x y HH. cdes HH.
-  apply seq_eqv_l. split; auto.
-  intros [z AA].
-  cdes STEP.
+  split; [|basic_solver].
+  intros x [[y AA] [z BB]].
   cdes AA.
+  cdes STEP.
+  cdes BB.
   rewrite <- ISTEP in ISTEP1. inv ISTEP1.
   inv ISTEP2.
   all: inv ISTEP0.
 Qed.
 
+Lemma ineps_step_stable_l thread lbls :
+  ineps_step thread lbls ≡ ⦗ stable_state thread ⦘ ⨾ ineps_step thread lbls.
+Proof.
+  split; [|basic_solver].
+  intros x y HH.
+  apply seq_eqv_l. split; auto.
+  intros [z AA].
+  eapply ineps_eps_step_dom_empty.
+  split; eexists; eauto.
+Qed.
+
+Lemma neps_step_stable_l thread :
+  neps_step thread ≡ ⦗ stable_state thread ⦘ ⨾ neps_step thread.
+Proof.
+  split; [|basic_solver].
+  intros x y HH.
+  apply seq_eqv_l. split; auto.
+  red in HH. desf.
+  apply ineps_step_stable_l in HH.
+  apply seq_eqv_l in HH. desf.
+Qed.
+
+Lemma lbl_step_alt thread :
+  lbl_step thread ≡ neps_step thread ⨾ (istep thread [])＊ ⨾ ⦗stable_state thread⦘.
+Proof.
+  split.
+  { intros x y [l [e HH]].
+    eexists. split; [eexists|]; apply HH. }
+  intros x y [e [[l AA] HH]].
+  eexists. eexists. split; eauto.
+Qed.
+
 Lemma steps_stable_lbl_steps thread :
   ⦗ stable_state thread ⦘ ⨾ (step thread)＊ ⨾ ⦗ stable_state thread ⦘ ⊆ (lbl_step thread)＊.
 Proof.
-Admitted.
+  arewrite (step thread ⊆ neps_step thread ∪ istep thread []).
+  { intros x y HH. red in HH. desf.
+    destruct lbls; [by right|].
+    left. eexists. red.
+      by splits; eauto. }
+  rewrite rt_unionE.
+  rewrite seqA.
+  arewrite (⦗stable_state thread⦘ ⨾ (istep thread [])＊ ⊆ ⦗stable_state thread⦘).
+  { rewrite rtE. rewrite seq_union_r.
+    apply inclusion_union_l; [basic_solver|].
+    rewrite ct_begin.
+    arewrite (⦗stable_state thread⦘ ⨾ istep thread [] ⊆ ∅₂).
+    2: basic_solver.
+    intros x y HH.
+    apply seq_eqv_l in HH. apply HH.
+    eexists. apply HH. }
+  rewrite rt_dom_ri.
+  2: { rewrite neps_step_stable_l at 1. by rewrite !seqA. }
+  rewrite !seqA.
+  rewrite <- lbl_step_alt.
+  basic_solver.
+Qed.
